need to do that for fin/Z/L

ETCSsorts.sml
@@ -1,0 +1,10 @@
+val _ = new_sort "ob" [] 
+val _ = new_sort "ar" [("A",mk_sort "ob" []),("B",mk_sort "ob" [])];
+val _ = EqSorts := "ar" :: (!EqSorts);
+val _ = new_sort_infix "ar" "->";
+val ob_sort = mk_sort "ob" [];
+fun ar_sort A B = mk_sort "ar" [A,B];
+
+
+fun mk_ob name = mk_var (name,ob_sort);
+fun mk_ar name dom cod = mk_var (name,ar_sort dom cod);
